src/Std/Data/Iterators/Lemmas/Combinators/Take.lean
@@ -83,4 +83,13 @@ theorem Iter.toArray_take_of_finite {α β} [Iterator α Id β] {n : Nat}
     (it.take n).toArray = it.toArray.take n := by
   rw [← toArray_toList, ← toArray_toList, List.take_toArray, toList_take_of_finite]
 
+@[simp]
+theorem Iter.toList_take_zero {α β} [Iterator α Id β]
+    [Finite (Take α Id β) Id]
+    [IteratorCollect (Take α Id β) Id Id] [LawfulIteratorCollect (Take α Id β) Id Id]
+    {it : Iter (α := α) β} :
+    (it.take 0).toList = [] := by
+  rw [toList_eq_match_step]
+  simp [step_take]
+
 end Std.Iterators
